tests/micro-benchmarks/TestQueue.fst
@@ -1,17 +1,23 @@
 module TestQueue
 open FStar.Queue
 
-let my_empty = as_queue []
-let my_queue = as_queue [1]
-let my_queue2 = as_queue #int [1; 2; 3]
+let my_queue = enqueue 3 (enqueue 2 (enqueue 1 empty))
 
-// let lemma_my_queue_not_empty : #a:Type -> Lemma (not_empty my_queue) = admit()
-
-#push-options "--print_implicits --print_universes --query_stats"
-let _ = assert (empty #bool == my_empty)
-let _ = assert (empty #int == my_empty)
-let _ = assert (equal (enqueue 2 my_queue) (as_queue [1; 2]))
-let _ = assert (dequeue my_queue == 1, as_queue [2; 3])
-let _ = assert (dequeue (enqueue 1 my_empty) == 1, my_empty)
-let _ = assert (peek my_queue == 1)
-let _ = assert (peek (snd (dequeue my_queue)) == 2)
+let _ = assert 
+  (eq my_queue
+      (as_queue [1; 2; 3]))
+let _ = assert 
+  (eq (enqueue 4 my_queue) 
+      (as_queue [1; 2; 3; 4]))
+let _ = assert 
+  (fst (dequeue my_queue) == 1)
+let _ = assert 
+  (eq (snd (dequeue my_queue)) 
+      (enqueue 3 (enqueue 2 empty)))
+let _ = assert 
+  (eq (snd (dequeue (enqueue 1 empty))) 
+      empty)
+let _ = assert 
+  (peek my_queue == 1)
+let _ = assert 
+  (peek (snd (dequeue my_queue)) == 2)
